low/RinternalsAux.v
@@ -302,56 +302,48 @@ Definition make_SExpRec_prim attrib prim type :=
       (make_PrimSxp_struct prim)).
 
 Definition make_SExpRec_char attrib array :=
-  let array := ArrayList.from_list array in
   SExpRec_VectorChar
     (make_Vector_SExpRec
       (build_SExpRecHeader CharSxp (decide (ArrayList.length array = 1)) attrib)
       (make_VecSxp_struct (ArrayList.length array) array)).
 
 Definition make_SExpRec_lgl attrib array :=
-  let array := ArrayList.from_list array in
   SExpRec_VectorLogical
     (make_Vector_SExpRec
       (build_SExpRecHeader LglSxp (decide (ArrayList.length array = 1)) attrib)
       (make_VecSxp_struct (ArrayList.length array) array)).
 
 Definition make_SExpRec_int attrib array :=
-  let array := ArrayList.from_list array in
   SExpRec_VectorInteger
     (make_Vector_SExpRec
       (build_SExpRecHeader IntSxp (decide (ArrayList.length array = 1)) attrib)
       (make_VecSxp_struct (ArrayList.length array) array)).
 
 Definition make_SExpRec_real attrib array :=
-  let array := ArrayList.from_list array in
   SExpRec_VectorReal
     (make_Vector_SExpRec
       (build_SExpRecHeader RealSxp (decide (ArrayList.length array = 1)) attrib)
       (make_VecSxp_struct (ArrayList.length array) array)).
 
 Definition make_SExpRec_cplx attrib array :=
-  let array := ArrayList.from_list array in
   SExpRec_VectorComplex
     (make_Vector_SExpRec
       (build_SExpRecHeader CplxSxp (decide (ArrayList.length array = 1)) attrib)
       (make_VecSxp_struct (ArrayList.length array) array)).
 
 Definition make_SExpRec_str attrib array :=
-  let array := ArrayList.from_list array in
   SExpRec_VectorPointer
     (make_Vector_SExpRec
       (build_SExpRecHeader StrSxp (decide (ArrayList.length array = 1)) attrib)
       (make_VecSxp_struct (ArrayList.length array) array)).
 
 Definition make_SExpRec_vec attrib array :=
-  let array := ArrayList.from_list array in
   SExpRec_VectorPointer
     (make_Vector_SExpRec
       (build_SExpRecHeader VecSxp (decide (ArrayList.length array = 1)) attrib)
       (make_VecSxp_struct (ArrayList.length array) array)).
 
 Definition make_SExpRec_expr attrib array :=
-  let array := ArrayList.from_list array in
   SExpRec_VectorPointer
     (make_Vector_SExpRec
       (build_SExpRecHeader ExprSxp (decide (ArrayList.length array = 1)) attrib)
